src/PlutusIR/Semantics/Static/typing_toy_let/toy_let.v
@@ -1,0 +1,52 @@
+Require Import Coq.Bool.Bool.
+Require Import Coq.Strings.String.
+Require Import Coq.Lists.List.
+Import ListNotations.
+
+From PlutusCert Require Import Util.List.
+
+Inductive ty := TyBool.
+
+Inductive term := 
+    | TBool : bool -> term
+    | TVar : string -> term
+    | TLet : TB -> term -> term
+    with TB := TBI : string -> ty -> term -> TB.
+
+Inductive has_type : list (string * ty) -> term -> ty -> Prop :=
+    | Ty_Bool : forall Γ b, has_type Γ (TBool b) TyBool
+    | Ty_Var : forall x Γ T, lookup x Γ = Some T -> has_type Γ (TVar x) T
+    | Ty_Let : forall x T_x t_x t T Γ, 
+        b_wf Γ (TBI x T_x t_x) ->
+        has_type ((x, T_x)::Γ) t T -> 
+        has_type Γ (TLet (TBI x T_x t_x) t) T
+with b_wf : list (string * ty) -> TB -> Prop :=
+    | W_term : forall Γ x T_x t_x, 
+        has_type Γ t_x T_x ->
+        b_wf Γ (TBI x T_x t_x).
+
+Definition b_wf_check (type_check : list (string * ty) -> term -> option ty) (Γ : list (string * ty)) (t : term) (T : ty) : bool :=
+    match type_check Γ t with
+    | Some T => true
+    | _ => false
+    end.
+
+Fixpoint type_check (Γ : list (string * ty))  (term : term) : option ty :=
+    match term with
+    | TBool b => Some TyBool
+    | TVar x => lookup x Γ
+    | TLet (TBI x T_x t_x) t => if b_wf_check type_check Γ t_x T_x then
+                                    type_check ((x, T_x)::Γ) t else None
+    end.
+
+Theorem type_check_complete Γ t T :
+    has_type Γ t T -> type_check Γ t = Some T.
+Proof.
+    intros.
+    induction H.
+    - admit.
+    - admit.
+    - simpl.
+      rewrite IHhas_type.
+      (* ????*)
+Admitted.
